examples/ijr/resolveFullyLib.sml
@@ -2,12 +2,13 @@ structure resolveFullyLib =
 struct
 open HolKernel Parse boolLib bossLib;
 
-open optionSyntax bir_htSyntax;
+open optionSyntax bir_htSyntax bir_wm_instSyntax;
 
 open bir_wp_interfaceLib;
 open tutorial_smtSupportLib;
 open bir_compositionLib;
 
+open listTheory;
 open resolveFullyTheory;
 open timersLib;
 
@@ -23,7 +24,7 @@ fun resolve_indirect_jumps(prog'_name, prog_tm, args) =
     (prog'_def, prog'_thm')
   end
 
-fun transfer_contract(prog'_thm, ht_thm) =
+fun transfer_bir_exec_to_labels_triple(prog'_thm, ht_thm) =
   let
     val prog_tm = (el 1 o snd o strip_comb o lhs o concl) prog'_thm
     val ht_tm = concl ht_thm
@@ -41,8 +42,37 @@ fun transfer_contract(prog'_thm, ht_thm) =
     MATCH_MP res_thm ht_thm
   end
 
+fun transfer_contract(prog'_thm, ht_thm) =
+  let
+    val prog_tm = (el 1 o snd o strip_comb o lhs o concl) prog'_thm
+    val ht_tm = concl ht_thm
+    val (_, _, entry_tm, wl_tm, bl_tm, _, _) = dest_bir_simp_jgmt ht_tm
+    val entry_thm = prove (
+      “MEM ^entry_tm (bir_labels_of_program ^prog_tm)”,
+      EVAL_TAC)
+    val wl_thm = prove (
+      “^wl_tm SUBSET (set (bir_labels_of_program ^prog_tm))”,
+      EVAL_TAC)
+    val bl_thm = prove (
+      “^bl_tm SUBSET (set (bir_labels_of_program ^prog_tm))”,
+      EVAL_TAC)
+    val res_thm = MATCH_MP resolve_fully_n_bir_simp_jgmt_transfer prog'_thm
+    val res_thm = MATCH_MP res_thm entry_thm
+    val res_thm = MATCH_MP res_thm wl_thm
+    val res_thm = MATCH_MP res_thm bl_thm
+  in
+    MATCH_MP res_thm ht_thm
+  end
+
 fun prove_and_transfer_contract(prog'_thm, prefix, pre_tm, entry_label_tm, ending_labels_tm, post_tm, defs) =
   let
+    (*Add exit points*)
+    val args_tm = (el 2 o snd o strip_comb o lhs o concl) prog'_thm
+    val bl_tm1 = EVAL “set (MAP (BL_Label o SND o LAST o SND) ^args_tm)”
+    val bl_tm2 = REWRITE_RULE [LIST_TO_SET] bl_tm1
+    val bl_tm3 = (rhs o concl) bl_tm2
+    val ending_labels_tm = (rhs o concl o EVAL) “^ending_labels_tm UNION ^bl_tm3”
+
     val wp_start = timer_start ()
     val prog'_tm = (dest_some o rhs o concl) prog'_thm
     (*Obtain WP contract*)
@@ -54,23 +84,27 @@ fun prove_and_transfer_contract(prog'_thm, prefix, pre_tm, entry_label_tm, endin
         prefix defs
     val _ = print ("WP time: " ^ timer_stop_str wp_start ^ "\n")
     
+    (*Simplify WP contract*)
     val wp_var = mk_var(prefix ^ "_wp", type_of wp_tm)
     val wp_def = Define `^(wp_var) = ^(wp_tm)`
     val ht_thm' = REWRITE_RULE [GSYM wp_def] ht_thm
     
-    (*Transfer WP contract*)
-    val transfer_start = timer_start ()
-    val ht'_thm = transfer_contract(prog'_thm, ht_thm')
-    val _ = print ("Transfer time: " ^ timer_stop_str transfer_start ^ "\n")
-
     (*Prove implication using SMT solvers*)
     val smt_start = timer_start ()
     val contract_imp = bimp (pre_tm, (lhs o concl) wp_def)
     val contract_imp_taut_thm = prove_exp_is_taut contract_imp
-    val res = label_ct_to_simp_ct_predset ht'_thm contract_imp_taut_thm
+    val contract = label_ct_to_simp_ct_predset ht_thm' contract_imp_taut_thm
     val _ = print ("SMT time: " ^ timer_stop_str smt_start ^ "\n")
+
+    (*Remove new exit points*)
+    val contract = bir_remove_labels_from_blist_predset contract bl_tm3
+
+    (*Transfer WP contract*)
+    val transfer_start = timer_start ()
+    val contract = transfer_contract(prog'_thm, contract)
+    val _ = print ("Transfer time: " ^ timer_stop_str transfer_start ^ "\n")
   in
-    res
+    contract
   end
 
 end
