examples/ijr/examplesScript.sml
@@ -24,7 +24,7 @@ val prog_def = bdefprog_list "prog" [block1, block2]
 val prog_tm = (lhs o concl) prog_def
 
 (*resolve_fail and resolve tests*)
-val resolve_fail_prog'_thm = EVAL “resolve_fail ^prog_tm (BL_Address (Imm64 0w)) (Imm64 4w)”
+val resolve_fail_prog'_thm = EVAL “resolve_fail ^prog_tm (BL_Address (Imm64 0w))”
 val resolve_fail_prog'_tm = (dest_some o rhs o concl) resolve_fail_prog'_thm
 
 val resolve_prog'_thm = EVAL “resolve ^prog_tm (BL_Address (Imm64 0w)) (Imm64 10w) "0w-1"”
@@ -34,13 +34,12 @@ val resolve_prog'_tm = (dest_some o rhs o concl) resolve_prog'_thm
 (*resolve_fully test*)
 val arg1 = “BL_Address (Imm64 0w)”
 val arg2 = “[(Imm64 10w, "0w-1"); (Imm64 4w, "0w-2")]”
-val arg3 = “Imm64 4w”
-val resolve_fully_prog'_thm = EVAL “resolve_fully ^prog_tm ^arg1 ^arg2 ^arg3”
+val resolve_fully_prog'_thm = EVAL “resolve_fully ^prog_tm ^arg1 ^arg2”
 val resolve_fully_prog'_tm = (dest_some o rhs o concl) resolve_fully_prog'_thm
 
 
 (*resolve_fully_n one indirect jump test many steps*)
-val resolve_fully_n_args = “[(^arg1, ^arg2, ^arg3)]”
+val resolve_fully_n_args = “[(^arg1, ^arg2)]”
 val resolve_fully_n_prog'_thm = EVAL “resolve_fully_n ^prog_tm ^resolve_fully_n_args”
 val resolve_fully_n_prog'_tm = (dest_some o rhs o concl) resolve_fully_n_prog'_thm
 
@@ -52,24 +51,25 @@ val block1' = (blabel_addr64 8,
 val prog2_def = bdefprog_list "prog2" [block1, block2, block1']
 val prog2_tm = (rhs o concl) prog2_def
 
-val prog2_args = “[(^arg1, ^arg2, ^arg3);
-             (BL_Address (Imm64 8w), [(Imm64 10w, "8w-1"); (Imm64 4w, "8w-2")], ^arg3)]”
+val prog2_args = “[(^arg1, ^arg2);
+                   (BL_Address (Imm64 8w), [(Imm64 10w, "8w-1"); (Imm64 4w, "8w-2")])]”
 val prog2'_thm = EVAL “resolve_fully_n ^prog2_tm ^prog2_args”
 val prog2'_tm = (dest_some o rhs o concl) prog2'_thm
 
 
 (*resolve_indirect_jumps and transfer_contract test*)
 (*Transform program*)
-val small_args = “[(BL_Address (Imm64 0w), [(Imm64 4w, "0w-2")], ^arg3)]”
+val small_args = “[(BL_Address (Imm64 0w), [(Imm64 4w, "0w-2")])]”
 val (small_prog'_def, small_prog'_thm) = 
   resolve_indirect_jumps("resolved_small_prog", prog_tm, small_args)
 
 (*Obtain WP contract*)
 val pre_def = Define ‘pre = bir_exp_true’
 val post_def = Define ‘post = ^(beq((bden o bvarimm64) "y", bconst64 4))’
-val prefix = "example1_"
+val prefix = "example1"
 val pre_tm = (lhs o concl) pre_def
 val entry_label_tm = “BL_Address (Imm64 0w)”
+
 val ending_labels_tm = “{BL_Address (Imm64 4w)}”
 val post_tm = “\l. if (l = BL_Address (Imm64 4w))
                    then post
@@ -91,9 +91,10 @@ val large_prog_args = gen_args_program(middle_blocks_n, 1)
 val (large_prog'_def, large_prog'_thm) = 
   resolve_indirect_jumps("resolved_large_prog", large_prog_tm, large_prog_args)
 
+
 val pre_def = Define ‘pre = ^(blt((bden o bvarimm64) "x", (bconst64 middle_blocks_n)))’
 val post_def = Define ‘post = ^(beq((bden o bvarimm64) "y", bconst64 exit_addr))’
-val prefix = "example2_"
+val prefix = "example2"
 val pre_tm = (lhs o concl) pre_def
 val entry_label_tm = “BL_Label "entry1"”
 val ending_labels_tm = “{^(blabel_addr64 exit_addr)}”
